[rp] lib/mult3 c-sum-merge measure proved, and guards verified without any skip proofs. But there are still some skip-proofs in the correctness proofs.

books/projects/rp-rewriter/lib/mult3/verify-guards.lisp
@@ -40,8 +40,1236 @@
 
 (include-book "summation-tree-meta-fncs")
 
-(skip-proofs
- (verify-guards c-sum-merge-fn))
+(local
+ (include-book "projects/rp-rewriter/proofs/rp-equal-lemmas" :dir :system))
+
+(local
+ (fetch-new-events
+  (include-book "arithmetic-5/top" :dir :system)
+  use-arith-5
+  :disabled t))
+
+(progn
+  (define lte (a b)
+    :verify-guards nil
+    (<= a b)
+    ///
+    (defthm rw-<=-to-lte
+      (equal (<= a b)
+             (lte a b))))
+
+  (define lt (a b)
+    :verify-guards nil
+    (< a b)
+    ///
+    (defthm rw-<-to-lte
+      (equal (< a b)
+             (lt a b))))
+
+  (define gt (a b)
+    :verify-guards nil
+    (> a b)
+    ///
+    (defthm rw->-to-gt
+      (equal (> a b)
+             (gt a b))))
+
+  (define gte (a b)
+    :verify-guards nil
+    (>= a b)
+    ///
+    (defthm rw->=-to-gte
+      (equal (>= a b)
+             (gte a b))))
+
+  (deftheory rw-dir1
+    '(rw-<-to-lte
+      rw->=-to-gte
+      rw->-to-gt
+      rw-<=-to-lte))
+
+  (deftheory rw-dir2
+    '(lt lte gte gt)))
+
+(local
+ (defthm ex-from-rp-loose-of-ex-from-rp
+   (equal (ex-from-rp (ex-from-rp term))
+          (ex-from-rp term))
+   :hints (("Goal"
+            :in-theory (e/d (ex-from-rp ex-from-rp
+                                        is-rp
+                                        is-rp)
+                            ())))))
+
+(local
+ (defthmd ex-from-rp-and-count-c-1
+   (and (equal (count-c (ex-from-rp c1))
+               (count-c c1)))
+   :hints (("Goal"
+            :expand (count-c (ex-from-rp c1))
+            :do-not-induct t
+            :in-theory (e/d (count-c
+                             count-c-lst)
+                            ())))))
+
+(local
+ (defthmd ex-from-rp-and-count-c-1-reverse
+   (implies (syntaxp (atom c1))
+            (and (equal (count-c c1)
+                        (count-c (ex-from-rp c1)))))
+   :hints (("Goal"
+            :expand (count-c (ex-from-rp c1))
+            :do-not-induct t
+            :in-theory (e/d (count-c
+                             count-c-lst)
+                            ())))))
+
+(local
+ (defthm ex-from-rp-and-count-c-2
+   (implies (and (equal (ex-from-rp c1)
+                        (ex-from-rp c2))
+                 (syntaxp (Not (lexorder c1 c2))))
+            (equal (count-c c1)
+                   (count-c c2)))
+   :hints (("Goal"
+            :do-not-induct t
+            :in-theory (e/d (ex-from-rp-and-count-c-1-reverse) ())))))
+
+(local
+ (defthmd  count-c-when-rp-equal-lemma
+   (implies (equal (car term) 'list)
+            (equal (ex-from-rp term)
+                   term))
+   :hints (("Goal"
+            :in-theory (e/d (ex-from-rp is-rp) ())))))
+
+;; (Local
+;;  (defthm count-c-when-rp-equal-2
+;;    (and (implies (and (RP-EQUAL TERM1 TERM2)
+;;                       (SINGLE-C-P (EX-FROM-RP TERM1)))
+;;                  (SINGLE-C-P (EX-FROM-RP TERM2))))
+;;    :rule-classes :forward-chaining
+;;    :hints (("Goal"
+;;             :expand ((RP-EQUAL TERM1 TERM2))
+;;             :in-theory (e/d (SINGLE-C-P)
+;;                             (RP-EQUAL))))))
+
+;; (Local
+;;  (defthm count-c-when-rp-equal-2.5
+;;    (and (implies (and (RP-EQUAL TERM1 TERM2)
+;;                       (not (SINGLE-C-P (EX-FROM-RP TERM1))))
+;;                  (not (SINGLE-C-P (EX-FROM-RP TERM2)))))
+;;    :rule-classes :forward-chaining
+;;    :hints (("Goal"
+;;             :expand ((RP-EQUAL TERM1 TERM2))
+;;             :in-theory (e/d (SINGLE-C-P)
+;;                             (RP-EQUAL))))))
+
+;; (Local
+;;  (defthm count-c-when-rp-equal-3
+;;    (implies (and (RP-EQUAL TERM1 TERM2)
+;;                  (SINGLE-s-P (EX-FROM-RP TERM1)))
+;;             (SINGLE-s-P (EX-FROM-RP TERM2)))
+;;    :rule-classes :forward-chaining
+;;    :hints (("Goal"
+;;             :expand ((RP-EQUAL TERM1 TERM2))
+;;             :in-theory (e/d (SINGLE-s-P)
+;;                             (RP-EQUAL))))))
+
+;; (Local
+;;  (defthm count-c-when-rp-equal-3.5
+;;    (and (implies (and (RP-EQUAL TERM1 TERM2)
+;;                       (not (SINGLE-s-P (EX-FROM-RP TERM1))))
+;;                  (not (SINGLE-s-P (EX-FROM-RP TERM2)))))
+;;    :rule-classes (:forward-chaining :rewrite)
+;;    :hints (("Goal"
+;;             :expand ((RP-EQUAL TERM1 TERM2))
+;;             :in-theory (e/d (SINGLE-s-P)
+;;                             (RP-EQUAL))))))
+
+;; (Local
+;;  (defthm count-c-when-rp-equal-4
+;;    (implies (and (RP-EQUAL TERM1 TERM2)
+;;                  (syntaxp (not (lexorder term1 term2))))
+;;             (and (iff (CONSP (EX-FROM-RP TERM1))
+;;                       (CONSP (EX-FROM-RP TERM2)))))
+;;    :rule-classes :forward-chaining
+;;    :hints (("Goal"
+;;             :expand ((RP-EQUAL TERM1 TERM2))
+;;             :in-theory (e/d ()
+;;                             (RP-EQUAL))))))
+
+;; (Local
+;;  (defthm count-c-when-rp-equal-5
+;;    (implies (and (RP-EQUAL TERM1 TERM2))
+;;             (EQUAL (CAR (EX-FROM-RP TERM1))
+;;                    (CAR (EX-FROM-RP TERM2))))
+;;    :rule-classes :forward-chaining
+;;    :hints (("Goal"
+;;             :expand ((RP-EQUAL TERM1 TERM2))
+;;             :in-theory (e/d ()
+;;                             (RP-EQUAL))))))
+
+;; (Local
+;;  (defthm count-c-when-rp-equal-6
+;;    (implies (and (RP-EQUAL TERM1 TERM2))
+;;             (RP-EQUAL-SUBTERMS (CDR (EX-FROM-RP TERM1))
+;;                                (CDR (EX-FROM-RP TERM2))))
+;;    :rule-classes :forward-chaining
+;;    :hints (("Goal"
+;;             :expand ((RP-EQUAL TERM1 TERM2))
+;;             :in-theory (e/d ()
+;;                             (RP-EQUAL))))))
+
+;; (Local
+;;  (defthm count-c-when-rp-equal-7
+;;    (implies (and (RP-EQUAL TERM1 TERM2)
+;;                  (single-s-p (EX-FROM-RP TERM1)))
+;;             (and (rp-equal (car (cdddr (EX-FROM-RP TERM1)))
+;;                            (car (cdddr (EX-FROM-RP TERM2))))))
+
+;;    :rule-classes :forward-chaining
+;;    :hints (("Goal"
+;;             :expand ((RP-EQUAL TERM1 TERM2))
+;;             :in-theory (e/d ()
+;;                             (RP-EQUAL))))))
+
+;; (Local
+;;  (defthm count-c-when-rp-equal-8
+;;    (implies (and (RP-EQUAL TERM1 TERM2)
+;;                  (single-c-p (EX-FROM-RP TERM1)))
+;;             (and (rp-equal (car (cddddr (EX-FROM-RP TERM1)))
+;;                            (car (cddddr (EX-FROM-RP TERM2))))))
+
+;;    :rule-classes :forward-chaining
+;;    :hints (("Goal"
+;;             :expand ((RP-EQUAL TERM1 TERM2))
+;;             :in-theory (e/d ()
+;;                             (RP-EQUAL))))))
+
+;; (local
+;;  (defthm-rp-equal-cnt
+;;    (defthm count-c-when-rp-equal
+;;      (implies (rp-equal-cnt term1 term2 cnt)
+;;               (equal (count-c term1)
+;;                      (count-c term2)))
+;;      :flag rp-equal-cnt)
+;;    (defthm count-c-lst-when-rp-equal-subterms
+;;      (implies (rp-equal-cnt-subterms subterm1 subterm2 cnt)
+;;               (equal (count-c-lst subterm1)
+;;                      (count-c-lst subterm2)))
+;;      :flag rp-equal-cnt-subterms)
+;;    :hints (("Goal"
+;;             :expand ((RP-EQUAL-SUBTERMS SUBTERM1 SUBTERM2)
+;;                      (COUNT-C (EX-FROM-RP TERM1))
+;;                      (COUNT-C (EX-FROM-RP TERM2)))
+;;             :do-not-induct t
+;;             :in-theory (e/d (ex-from-rp-and-count-c-1-reverse
+;;                              count-c-when-rp-equal-lemma
+;;                              count-c-lst
+;;                              count-c)
+;;                             (RP-EQUAL-IS-SYMMETRIC
+;;                              count-c-when-rp-equal-7
+;;                              count-c-when-rp-equal-8
+;;                              rp-equal-subterms
+;;                              rp-equal
+;;                              RP-EQUAL-SUBTERMS-IS-SYMMETRIC)))
+;;            ("Subgoal *1/10"
+;;             :use ((:instance count-c-when-rp-equal-7)
+;;                   (:instance count-c-when-rp-equal-8))))))
+
+(local
+ (std::defret
+  measure-lemma-of-cough-duplicates
+  ;; (equal (+ (count-c-lst coughed-lst)
+  ;;           (count-c-lst coughed-lst)
+  ;;           (count-c-lst res-lst))
+  ;;        (count-c-lst lst))
+  (and #|(implies (consp lst)
+   (and (lt (count-c-lst COUGHED-LST)
+   (count-c-lst lst))
+   (not (gte (count-c-lst COUGHED-LST)
+   (count-c-lst lst)))))||#
+   (lte (count-c-lst COUGHED-LST)
+        (count-c-lst lst))
+   (not (gt (count-c-lst COUGHED-LST)
+            (count-c-lst lst)))
+   (lte (count-c-lst RES-LST)
+        (count-c-lst lst))
+   (not (gt (count-c-lst RES-LST)
+            (count-c-lst lst)))
+   (lte (+ (count-c-lst COUGHED-LST)
+           (count-c-lst RES-LST))
+        (count-c-lst lst))
+   (not (gt (+ (count-c-lst COUGHED-LST)
+               (count-c-lst RES-LST))
+            (count-c-lst lst))))
+  :fn COUGH-DUPLICATES
+  :hints (("Goal"
+           :do-not-induct t
+           :induct (COUGH-DUPLICATES lst)
+           :in-theory (e/d (COUNT-C-LST
+                            rw-dir2
+                            COUGH-DUPLICATES)
+                           (rw-dir1))))))
+
+(local
+ (defthm ex-from-rp-loose-of-cons
+   (implies (not (equal fnc 'rp))
+            (equal (ex-from-rp (cons fnc rest))
+                   (cons fnc rest)))
+   :hints (("Goal"
+            :in-theory (e/d (ex-from-rp
+                             is-rp)
+                            ())))))
+
+(set-ignore-ok t)
+(local
+ (make-event
+  (b* ((count-c-formula (meta-extract-formula 'count-c state))
+       (count-c-formula (caddr count-c-formula)))
+    `(defthm count-c-when-c-instance
+       (equal (count-c (cons 'c args))
+              (let ((term (cons 'c args)))
+                ,count-c-formula))
+       :hints (("Goal"
+                :in-theory (e/d (count-c) ())))))))
+
+(local
+ (defthm count-c-when-quoted
+   (equal (count-c (cons 'quote rest))
+          0)
+   :hints (("Goal"
+            :expand ((count-c (cons 'quote rest))
+                     (ex-from-rp (CONS 'QUOTE REST)))
+            :in-theory (e/d (count-c
+                             single-c-p
+                             single-s-p)
+                            ())))))
+
+
+(local
+ (defthm local-measure-lemma-1
+   (implies (and (acl2-numberp a)
+                 (acl2-numberp b))
+            (and (equal (< (1+ a) (1+ b))
+                        (< a b))
+                 (equal (lt (1+ a) (1+ b))
+                        (lt a b))
+                 (equal (> (1+ a) (1+ b))
+                        (> a b))
+                 (equal (gt (1+ a) (1+ b))
+                        (gt a b))
+                 (equal (> (+ a 1) (+ b 1))
+                        (> a b))
+                 (equal (gt (+ a 1) (+ b 1))
+                        (gt a b))
+                 (equal (< (+ a 1) (+ b 1))
+                        (< a b))
+                 (equal (lt (+ a 1) (+ b 1))
+                        (lt a b))
+                 (equal (<= (1+ a) (1+ b))
+                        (<= a b))
+                 (equal (lte (1+ a) (1+ b))
+                        (lte a b))
+                 (equal (>= (1+ a) (1+ b))
+                        (>= a b))
+                 (equal (gte (1+ a) (1+ b))
+                        (gte a b))))
+   :hints (("Goal"
+            :in-theory (e/d (rw-dir2
+                             (:REWRITE ACL2::|(+ y x)|)
+                             (:REWRITE ACL2::|(equal (if a b c) x)|)
+                             (:REWRITE ACL2::EQUAL-OF-PREDICATES-REWRITE))
+                            (rw-dir1))))))
+
+
+
+(local
+ (defthm local-measure-lemma-2
+   (and (implies (and (<= a b)
+                      (<= b c))
+                 (<= a c))
+        (implies (and (lte a b)
+                      (lte b c))
+                 (and (lte a c)
+                      (not (gt a c))))
+        (implies (and (gte a b)
+                      (gte b c))
+                 (and (gte a c)
+                      (not (lt a c))))
+        (implies (and (lt a b)
+                      (lte b c))
+                 (and (lt a c)
+                      (not (gte a c))))
+        (implies (and (lte a b)
+                      (lt b c))
+                 (and (not (gte a c))
+                      (lt a c))))
+   :hints (("Goal"
+            :in-theory (e/d (rw-dir2)
+                            (rw-dir1))))
+   ))
+
+(local
+ (defthm local-measure-lemma-4
+   (and (lte a a)
+        (gte a a)
+        (not (gt a a))
+        (not (lt a a)))
+   :hints (("Goal"
+            :in-theory (e/d (rw-dir2)
+                            (rw-dir1))))))
+
+(local
+ (defthm count-c-lst-when-not-conp
+   (implies (atom x)
+            (equal (count-c-lst x)
+                   0))
+   :hints (("Goal"
+            :in-theory (e/d (count-c-lst) ())))))
+
+(local
+ (std::defret
+  measure-lemma-of-SWAP-C-LSTS
+  (and (equal (+ (count-c-lst res1)
+                 (count-c-lst res2))
+              (+ (count-c-lst c1-lst)
+                 (count-c-lst c2-lst)))
+       (equal (+ (count-c-lst res2)
+                 (count-c-lst res1))
+              (+ (count-c-lst c1-lst)
+                 (count-c-lst c2-lst)))
+       (implies (not res1)
+                (equal (count-c-lst res2)
+                       (+ (count-c-lst c1-lst)
+                          (count-c-lst c2-lst))))
+       (implies (not res2)
+                (equal (count-c-lst res1)
+                       (+ (count-c-lst c1-lst)
+                          (count-c-lst c2-lst)))))
+  :fn SWAP-C-LSTS
+  :hints (("Goal"
+           :in-theory (e/d (SWAP-C-LSTS) ())))))
+
+(local
+ (std::defret measure-lemma-of-s-sum-merge-aux
+              (and (lte (count-c-lst merged-s-lst)
+                        (+ (count-c-lst s1-lst)
+                           (count-c-lst s2-lst)))
+                   (not (gt (count-c-lst merged-s-lst)
+                            (+ (count-c-lst s1-lst)
+                               (count-c-lst s2-lst))))
+                   (<= (count-c-lst merged-s-lst)
+                       (+ (count-c-lst s1-lst)
+                          (count-c-lst s2-lst))))
+              :fn S-SUM-MERGE-AUX
+              :hints (("Goal"
+                       :in-theory (e/d (rw-dir2
+                                        COUNT-C-LST
+                                        S-SUM-MERGE-AUX)
+                                       (rw-dir1))))))
+
+(local
+ (defthm local-measure-lemma-5
+   (and (implies (and (lte a b)
+                      (lte b c)
+                      (lte c d))
+                 (and (lte a d)
+                      (not (gt a d)))))
+   :hints (("Goal"
+            :in-theory (e/d (rw-dir2) (rw-dir1))))))
+
+(local
+ (defthm local-measure-lemma-6
+   (implies (consp c1-lst)
+            (LTE (+ (COUNT-C-LST C2-LST)
+                    (COUNT-C (CAR C1-LST)))
+                 (+ (COUNT-C-LST C1-LST)
+                    (COUNT-C-LST C2-LST))))
+   :hints (("Goal"
+            :expand (COUNT-C-LST C1-LST)
+            :in-theory (e/d (rw-dir2 count-c-lst) (rw-dir1))))))
+(local
+ (defthm dummy-lemma1
+   (implies (and (natp a)
+                 (natp b))
+            (and
+             (lte a
+                  (+ a b))
+             (lte b
+                  (+ a b))))
+   :hints (("Goal"
+            :in-theory (e/d (rw-dir2) (rw-dir1))))))
+
+#|(local
+ (defthm gt-to-not-lte
+   (and (equal (gt a b)
+               (not (lte a b)))
+        (equal (gte a b)
+               (not (lt a b))))
+   :hints (("Goal"
+            :in-theory (e/d (rw-dir2) (rw-dir1))))))||#
+
+;; (local
+;;  (defthm bind-free-test
+;;    (implies (and (
+
+(local
+ (defthm dummy-lemma2
+   (implies (and (consp C1-LST)
+                 (acl2-numberp c))
+            (equal (gt (+ (COUNT-C-LST C1-LST) b)
+                       (+ (COUNT-C-LST (cdr C1-LST)) c))
+                   (gt (+ (COUNT-C (car C1-LST)) b)
+                       c)))
+   :hints (("Goal"
+            :use ((:instance ACL2::SIMPLIFY-SUMS-<
+                             (ACL2::X (COUNT-C-lst (cdr C1-LST)))
+                             (ACL2::RHS (+ (COUNT-C (car C1-LST)) b))
+                             (ACL2::LHS c)))
+            :Expand (COUNT-C-LST C1-LST)
+            :in-theory (e/d (rw-dir2)
+                            (rw-dir1))))))
+
+(local
+ (defthm dummy-lemma3
+   (implies (and (lte a b)
+                 (ACL2-NUMBERP a)
+                 (ACL2-NUMBERP b)
+                 (lte b a))
+            (equal a b))
+   :rule-classes :forward-chaining
+   :hints (("Goal"
+            :in-theory (e/d (rw-dir2) (rw-dir1))))))
+
+(local
+ (defthm dummy-lemma4
+   (implies (and (lte a b)
+                 (NOT (lte b a)))
+            (LT a b))
+   :rule-classes :forward-chaining
+   :hints (("Goal"
+            :in-theory (e/d (rw-dir2) (rw-dir1))))))
+
+#|(local
+ (defthm local-measure-lemma-3
+   (and (equal (not (gte a b))
+               (lt a b))
+        (equal (equal (gte a b) nil)
+               (lt a b))
+        (equal (iff (gte a b) nil)
+               (lt a b))
+        (equal (if (gte a b) nil t)
+               (lt a b))
+        (iff (not (gte a b))
+             (lt a b))
+
+        (equal (not (lte a b))
+               (gt a b))
+        (equal (if (lte a b) nil t)
+               (gt a b))
+        (iff (not (lte a b))
+             (gt a b))
+
+        (equal (not (lt a b))
+               (gte a b))
+        (equal (if (lt a b) nil t)
+               (gte a b))
+        (iff (not (lt a b))
+             (gte a b))
+
+        ;; (equal (gt a b)
+        ;;        (not (lte a b)))
+
+        ;; (equal (gte a b)
+        ;;        (not (lt a b)))
+
+        (equal (not (gt a b))
+               (lte a b))
+        (equal (equal (gt a b) nil)
+               (lte a b))
+        (equal (iff (gt a b) nil)
+               (lte a b))
+        (equal (if (gt a b) nil t)
+               (lte a b))
+        (iff (not (gt a b))
+             (lte a b))
+        (equal (or (gt a b) c)
+               (or (not (lte a b)) c))
+        )
+   :hints (("Goal"
+            :in-theory (e/d (rw-dir2)
+                            (rw-dir1))))))||#
+
+(local
+ (defthm local-measure-lemma-3-2
+   (AND (IMPLIES (ACL2::rewriting-positive-literal `(lt ,a ,b))
+                 (equal (lt a b)
+                        (NOT (gte a b))))
+        (IMPLIES (ACL2::rewriting-positive-literal `(Gt ,a ,b))
+                 (equal (gt a b)
+                        (NOT (lte a b))))
+        (IMPLIES (ACL2::rewriting-positive-literal `(gte ,a ,b))
+                 (equal (gte a b)
+                        (NOT (gt b a))))
+        (IMPLIES (ACL2::rewriting-positive-literal `(lte ,a ,b))
+                 (equal (lte a b)
+                        (NOT (gt a b)))))
+   :hints (("Goal"
+            :in-theory (e/d (rw-dir2)
+                            (rw-dir1))))))
+
+(local
+ (defthm dummy-lemma-5
+   (implies (ACL2-NUMBERP B)
+            (and (equal (lte (+ b a)
+                             (+ c d a))
+                        (lte b
+                             (+ c d)))
+                 (equal (lte (+ a b)
+                             (+ c d a))
+                        (lte b
+                             (+ c d)))))
+   :hints (("Goal"
+            :use ((:instance ACL2::SIMPLIFY-SUMS-<
+                             (ACL2::X a)
+                             (ACL2::RHS (+ c d))
+                             (ACL2::LHS b)))
+            :in-theory (e/d (rw-dir2) (rw-dir1))))))
+
+(defthm lte-and-gte-implies
+  (and (implies (lt x y)
+                (and (lte x y)
+                     (not (gt x y))))
+       (implies (gt x y)
+                (and (gte x y)
+                     (not (gt y x)))))
+  :hints (("Goal"
+           :in-theory (e/d (rw-dir2) (rw-dir1)))))
+
+(local
+ (defthm expand-count-c-lst-when-consp
+   (implies (consp x)
+            (equal (count-c-lst x)
+                   (+ (count-c (car x))
+                      (count-c-lst (cdr x)))))
+   :hints (("Goal"
+            :expand (count-c-lst x)
+            :in-theory (e/d () ())))))
+
+(local
+ (defthm count-c-of-quoted
+   (implies (EQUAL (CAR SINGLE-C1) 'QUOTE)
+            (equal (COUNT-C SINGLE-C1)
+                   0))
+   :hints (("Goal"
+            :in-theory (e/d (count-c) ())))))
+
+(local
+ (defthm dummy-lemma-6
+   (NOT (GT (COUNT-C-LST C2-LST)
+            (+ 1 (COUNT-C-LST C2-LST))))
+   :hints (("Goal"
+            :in-theory (e/d (rw-dir2) (rw-dir1))))))
+
+(local
+ (defthm dummy-lemma-7
+   (implies (acl2-numberp m)
+            (and (equal (lte (+ x a y)
+                             (+ a m))
+                        (lte (+ x y)
+                             m))
+                 (equal (lte (+ x y a)
+                             (+ a m))
+                        (lte (+ x y)
+                             m))
+                 (equal (gt (+ a m)
+                            (+ x y a))
+                        (gt m
+                            (+ x y)))))
+   :hints (("Goal"
+            :use ((:instance ACL2::SIMPLIFY-SUMS-<
+                             (ACL2::X a)
+                             (ACL2::rHS (+ x y))
+                             (ACL2::lHS m))
+                  (:instance ACL2::SIMPLIFY-SUMS-<
+                             (ACL2::X a)
+                             (ACL2::lHS (+ x y))
+                             (ACL2::rHS m)))
+            :in-theory (e/d (rw-dir2) (rw-dir1))))))
+
+
+
+(progn
+  (local
+   (defthm count-c-GET-C-ARGS-1
+     (and
+      (implies (and (MV-NTH 4 (GET-C-ARGS SINGLE-C1))
+                    ;;(case-split (not (equal (ex-from-rp SINGLE-C1) ''0)))
+                    )
+               (equal (COUNT-C-LST (MV-NTH 3 (GET-C-ARGS SINGLE-C1)))
+                      (1- (count-c SINGLE-C1)))))
+     :hints (("Goal"
+              :do-not-induct t
+              :expand (COUNT-C SINGLE-C1)
+              :in-theory (e/d (GET-C-ARGS
+                               SINGLE-C-P
+                               SINGLE-s-P)
+                              ())))))
+
+  #|(local
+  (defthm count-c-GET-C-ARGS-2
+  (and
+  (implies (and (MV-NTH 4 (GET-C-ARGS SINGLE-C1))
+  (CONSP (MV-NTH 1 (GET-C-ARGS SINGLE-C1)))
+  (EQUAL (CAR (MV-NTH 1 (GET-C-ARGS SINGLE-C1)))
+  'LIST))
+  (equal (COUNT-C-LST (MV-NTH 3 (GET-C-ARGS SINGLE-C1)))
+  (1- (count-c SINGLE-C1)))))
+  :hints (("Goal"
+  :do-not-induct t
+  :expand (COUNT-C SINGLE-C1)
+  :in-theory (e/d (GET-C-ARGS
+  SINGLE-C-P
+  SINGLE-s-P)
+  ())))))||#
+
+  #| (local
+  (defthm GET-C-ARGS-lemma1
+  (implies (EQUAL (EX-FROM-RP SINGLE-C1) ''0)
+  (equal (GET-C-ARGS SINGLE-C1)
+  (MV 0 ''NIL ''NIL NIL 'C)))
+  :hints (("Goal"
+  :in-theory (e/d (GET-C-ARGS) ())))))||#)
+
+(local
+ (defthm c-sum-merge-nil-lemma
+   (equal (C-SUM-MERGE NIL arg2
+                       :AUTO-SWAP T
+                       :CLEAN-C1-LST NIL)
+          (LIST* ''NIL NIL ARG2 '(NIL)))
+   :hints (("Goal"
+            :expand ((SWAP-C-LSTS NIL ARG2 T)
+                     (C-SUM-MERGE NIL arg2
+                                  :AUTO-SWAP T
+                                  :CLEAN-C1-LST NIL)
+                     (C-SUM-MERGE-AUX NIL ARG2
+                                      :CLEAN-C1-LST NIL)
+                     (C-SUM-MERGE-AUX ARG2 NIL
+                                      :CLEAN-C1-LST NIL))
+            :in-theory (e/d () ())))))
+
+;; (local
+;;  (defthm SINGLE-C-TRY-MERGE-PARAMS-lemma
+;;    (equal (SINGLE-C-TRY-MERGE-PARAMS s-lst
+;;                                      0 ''NIL
+;;                                      ''NIL
+;;                                      NIL)
+
+(local
+ (defthm dummy-lemma-8
+   (equal (lte a (+ -2 b))
+          (lte (+ a 2) b))
+   :hints (("Goal"
+            :in-theory (e/d (rw-dir2) (rw-dir1))))))
+
+(local
+ (defthm dummy-lemma-9
+   (implies (and (MV-NTH 4 (GET-C-ARGS SINGLE-C2)))
+            (consp single-c2))
+   :rule-classes :forward-chaining
+   :hints (("Goal"
+            :in-theory (e/d (GET-C-ARGS) ())))))
+
+(local
+ (defthm dummy-lemma-10
+   (implies (acl2-numberp b)
+            (and (equal (lte (+ 2 a x)
+                             (+ x b))
+                        (lte (+ 2 a)
+                             b))
+                 (equal (gt (+ 2 a x)
+                            (+ x b))
+                        (gt (+ 2 a)
+                            b))
+                 (equal (gte (+ 2 a x)
+                             (+ x b))
+                        (gte (+ 2 a)
+                             b))
+                 (equal (lt (+ 2 a x)
+                            (+ x b))
+                        (lt (+ 2 a)
+                            b))))
+   :hints (("Goal"
+            :use ((:instance ACL2::SIMPLIFY-SUMS-<
+                             (ACL2::X x)
+                             (ACL2::RHS (+ 2 a))
+                             (ACL2::LHS b))
+                  (:instance ACL2::SIMPLIFY-SUMS-<
+                             (ACL2::X x)
+                             (ACL2::LHS (+ 2 a))
+                             (ACL2::RHS b)))
+            :in-theory (e/d (rw-dir2) (rw-dir1))))))
+
+(local
+ (defthm dummy-lemma-11
+   (implies (lte a (1+ b))
+            (lte a (+ 2 b)))
+   :hints (("Goal"
+            :in-theory (e/d (rw-dir2) (rw-dir1))))))
+
+;; (local
+;;  (defthm dummy-lemma-12
+;;    (implies (lte a b)
+;;             (not (lte b a)))
+
+(progn
+
+  (local
+   (define lte-chain-smart-fn-aux (cl a d)
+     (if (or (atom cl)
+             )
+         (mv nil nil)
+       (b* ((cur (car cl))
+            ((mv rest-b rest-c)
+             (lte-chain-smart-fn-aux (cdr cl) a d))
+            ((unless (case-match cur (('not &) t)))
+             (mv rest-b rest-c))
+            (cur (cadr cur)))
+         (case-match cur
+           (('lte x y)
+            (mv (if (and (equal x a) (not (equal y d))) y rest-b)
+                (if (and (equal y d) (not (equal x a))) x rest-c)))
+           (('gt y x)
+            (mv (if (and (or (not rest-b) (equal rest-c d)) (equal x a) )
+                    (progn$   y)
+                  rest-b)
+                (if (and (or (not rest-c) (equal rest-c a)) (equal y d) )
+                    (progn$   x)
+                  rest-c)))
+           (&
+            (mv rest-b rest-c)))))))
+
+  (local
+   (define lte-chain-smart-fn (a d mfc state)
+     :verify-guards nil
+     (b* ( ;(ancestors  (mfc-ancestors mfc))
+          (rcnst (access acl2::metafunction-context mfc :rcnst))
+          (cl (access acl2::rewrite-constant rcnst :current-clause))
+          (?top-cl (access acl2::rewrite-constant rcnst :top-clause))
+          (cl (beta-search-reduce-subterms cl (expt 2 30)))
+          ((mv b c)
+           (lte-chain-smart-fn-aux cl a d))
+          ;;(- (cw "rcnst : ~p0 ~%" (cddr rcnst)))
+          (b (if (not b) c b))
+          (c (if (not c) b c))
+
+          #|(- (and (or (and b c)
+          (equal a '(binary-+
+          (COUNT-C-LST
+          (MV-NTH '0
+          (COUGH-DUPLICATES (MV-NTH '2 (C-SUM-MERGE-LST-LST C1-LST 'NIL)))))
+          (COUNT-C-LST
+          (MV-NTH
+          '1
+          (COUGH-DUPLICATES (MV-NTH '2 (C-SUM-MERGE-LST-LST C1-LST 'NIL))))))))
+          (cw "a: ~p0
+          b:~p1
+          c:~p2
+          d:~p3
+          cl:~p4
+          "
+          a b c d cl
+          )))||#)
+       (if (and b c)
+           (progn$
+;(cw "a:~p0 b:~p1 c:~p2, d:~p3 ~%" a b c d)
+            `((b . ,b)
+              (c . ,c)))
+         nil))))
+
+  (local
+   (defthm ge-chain-smart
+     (implies (and (bind-free (lte-chain-smart-fn a d mfc state)
+                              (b c))
+                   (or (and (gt b a)
+                            (gt c b)
+                            (gt d c))
+
+                       (and (gt b a)
+                            (gte c b)
+                            (gte d c))
+                       (and (gte b a)
+                            (gte c b)
+                            (gt d c))
+                       (and (gte b a)
+                            (gt c b)
+                            (gte d c))
+
+                       (and (gte b a)
+                            (gt c b)
+                            (gt d c))
+                       (and (gt b a)
+                            (gte c b)
+                            (gt d c))
+                       (and (gt b a)
+                            (gt c b)
+                            (gte d c)))
+                   )
+              (and ;(gt d a)
+               (not (lte d a))))
+     :hints (("Goal"
+              :in-theory (e/d (rw-dir2) (rw-dir1))))))
+
+  (local
+   (defthm lte-chain-smart
+     (implies (and (bind-free (lte-chain-smart-fn a d mfc state)
+                              (b c))
+                   (or (and (lte a b)
+                            (lte b c)
+                            (lte c d))
+
+                       (and (lte a b)
+                            (lte b c)
+                            (lt c d))
+                       (and (lte a b)
+                            (lt b c)
+                            (lte c d))
+                       (and (lt a b)
+                            (lte b c)
+                            (lte c d))
+
+                       (and (lt a b)
+                            (lte b c)
+                            (lt c d))
+                       (and (lte a b)
+                            (lt b c)
+                            (lt c d))
+                       (and (lt a b)
+                            (lt b c)
+                            (lte c d)))
+                   )
+              (and ;(lte a d)
+               (not (gt a d))))
+     :hints (("Goal"
+              :in-theory (e/d (rw-dir2) (rw-dir1))))))
+
+  )
+
+(local
+ (defthm gte-to-lte
+   (equal (gte a b)
+          (lte b a))
+   :hints (("Goal"
+            :in-theory (e/d (rw-dir2) (rw-dir1))))))
+
+
+(local
+ (defthm dummy-lemma-13
+   (implies (EQUAL (CAR C) 'LIST)
+            (NOT (GT (COUNT-C-LST (CDR C)) (COUNT-C C))))
+   :hints (("Goal"
+            :expand (COUNT-C C)
+            :in-theory (e/d (SINGLE-C-P
+                             EX-FROM-RP
+                             is-rp
+                             ) ())))))
+
+(local
+ (std::defret
+  measure-lemma-compress-s-c
+  (equal (count-c res-term)
+         (count-c term))
+  :fn compress-s-c
+  :hints (("Goal"
+           :induct (compress-s-c term :limit limit)
+           :do-not-induct t
+           :in-theory (e/d (compress-s-c
+                            count-c
+                            single-c-p
+                            single-s-p
+                            )
+                           ())))))
+(local
+ (defthm dummy-lemma-14
+   (implies (and (acl2-numberp a)
+                 (acl2-numberp b))
+            (equal (equal (+ 1 a) (+ 1 b))
+                   (equal a b)))))
+
+(local
+ (std::defret
+  measure-lemma-decompress-s-c
+  (equal (count-c res-term)
+         (count-c term))
+  :fn decompress-s-c
+  :hints (("Goal"
+           :induct (decompress-s-c term :limit limit)
+           :do-not-induct t
+           :in-theory (e/d (decompress-s-c
+                            CREATE-LIST-INSTANCE
+                            count-c
+                            single-c-p
+                            single-s-p
+                            )
+                           ())))))
+(local
+ (defthm dummy-lemma-15
+   (and (implies (and (equal (car c) 'list)
+                      (consp c))
+                 (equal (count-c c) (count-c-lst (cdr c)))))
+   :hints (("Goal"
+            :expand (count-c c)
+            :in-theory (e/d (EX-FROM-RP
+                             is-rp)
+                            ())))))
+
+(local
+ (defthm dummy-lemma-16
+   (and (implies (case-match term
+                   (('c & & & ('list . &)) t)
+                   (('c & & & ''nil) t))
+                 (and (equal (count-c (car (cddddr term)))
+                             (1- (count-c term)))
+                      (equal (count-c-lst (cdr (car (cddddr term))))
+                             (1- (count-c term)))))
+        (implies (case-match term
+                   (('c & & & ('list  &)) t))
+                 (and (equal (count-c (cadr (car (cddddr term))))
+                             (1- (count-c term))))))
+   :hints (("Goal"
+            :expand (count-c term)
+            :in-theory (e/d (EX-FROM-RP
+                             single-c-p
+                             is-rp)
+                            ())))))
+
+(local
+ (defthm dummy-lemma-17
+   (and (implies (acl2-numberp a)
+                 (not (gt (1- a) a)))
+        (implies (and (CONSP C)
+                      (EQUAL (CAR C) 'LIST)
+                      (CONSP (CDR C))
+                      (CONSP (CADR C))
+                      (EQUAL (CAR (CADR C)) 'C)
+                      (CONSP (CDR (CADR C)))
+                      (CONSP (CDDR (CADR C)))
+                      (EQUAL (CADDR (CADR C)) ''NIL)
+                      (CONSP (CDDDR (CADR C)))
+                      (CONSP (CDDDDR (CADR C)))
+                      (NOT (CDDR C))
+                      (NOT (CDR (CDDDDR (CADR C)))))
+                 (not (gt 0 (count-c (cadr c))))))
+  
+   :hints (("Goal"
+            :in-theory (e/d (rw-dir2) (rw-dir1))))))
+
+(local
+ (std::defret
+  measure-lemma-c-pattern2-reduce
+  (and (lte (count-c c-res)
+            (count-c c))
+       (<= (count-c c-res)
+           (count-c c))
+       (implies (case-match c-res (('list . &) t))
+                (lte (count-c-lst (cdr c-res))
+                     (count-c c)))
+       (implies (case-match c-res (('list . &) t))
+                (<= (count-c-lst (cdr c-res))
+                    (count-c c))))
+  :fn c-pattern2-reduce
+  ;:otf-flg t
+  :hints (("goal"
+           :do-not-induct t
+           :expand ((:free (x) (SINGLE-C-P `(c . ,x))))
+           :in-theory (e/d (c-pattern2-reduce
+                            count-c
+                            count-c-lst)
+                           (ex-from-rp))))))
+
+(local
+ (std::defret
+  measure-lemma-create-c-instance
+  (and (not (gt (count-c c-res)
+                (1+ (count-c c))))
+       (lte (count-c c-res)
+            (1+ (count-c c))))
+  :fn CREATE-C-INSTANCE
+  :hints (("Goal"
+           :in-theory (e/d (CREATE-C-INSTANCE
+                            SINGLE-C-P
+                            rw-dir2)
+                           (rw-dir1))))))
+
+(local
+ (std::defret measure-lemma-create-c-instance-2
+              (and (not (gte (count-c c-res)
+                             (+ 2 (count-c c))))
+                   (lt (count-c c-res)
+                       (+ 2 (count-c c)))
+                   (gt (+ 2 (count-c c))
+                       (count-c c-res)))
+              :fn CREATE-C-INSTANCE
+              :hints (("Goal"
+                       :use ((:instance measure-lemma-create-c-instance))
+                       :in-theory (e/d (rw-dir2) (rw-dir1
+                                                  measure-lemma-create-c-instance))))))
+
+(local
+ (defthm CREATE-list-INSTANCE-measure-lemma
+   (equal (count-c (create-list-instance lst))
+          (count-c-lst lst))
+   :hints (("Goal"
+            :expand (COUNT-C (CONS 'LIST LST))
+            :in-theory (e/d (create-list-instance
+                             SINGLE-S-P
+                             SINGLE-C-P)
+                            ())))))
+
+(local
+ (defthm
+   measure-lemma-create-c-instance-3
+   (b* ((c (create-list-instance c-lst))
+        (?c-res (create-c-instance s pp c)))
+     (and (not (gte (count-c c-res) (+ 2 (count-c-lst c-lst))))
+          (lt (count-c c-res) (+ 2 (count-c-lst c-lst)))
+          (gt (+ 2 (count-c-lst c-lst)) (count-c c-res))
+          (not (gt (count-c c-res)
+                   (1+ (count-c-lst c-lst))))
+          (lte (count-c c-res)
+               (1+ (count-c-lst c-lst)))))
+   :hints
+   (("goal" :use ((:instance measure-lemma-create-c-instance
+                             (c (create-list-instance c-lst))))
+     :in-theory
+     (e/d (rw-dir2)
+          (rw-dir1
+           measure-lemma-create-c-instance))))))
+
+
+
+(std::defret-mutual
+ measure-lemma-of-c-sum-merge
+ (std::defret
+  measure-lemma-of-single-c-try-merge
+  (implies merge-success
+           (and (< (count-c-lst produced-c-lst)
+                   (+ (count-c single-c1)
+                      (count-c single-c2)))
+                (consp single-c1)
+                (consp single-c2)))
+  :fn single-c-try-merge)
+ (std::defret
+  measure-lemma-of-c-sum-merge-lst-aux
+  (and (implies merge-success
+                (and (< (+ (count-c-lst produced-c-lst)
+                           (count-c-lst updated-c2-lst))
+                        (+ (count-c single-c1)
+                           (count-c-lst c2-lst)))
+                     (consp single-c1)))
+       (implies (not merge-success)
+                (and (equal produced-c-lst nil)
+                     (equal updated-c2-lst c2-lst))))
+  :fn c-sum-merge-lst-aux)
+ (std::defret
+  measure-lemma-of-c-sum-merge-lst
+  (<= (count-c-lst new-c2-lst)
+      (+ (count-c single-c1)
+         (count-c-lst c2-lst)))
+  :fn c-sum-merge-lst)
+ (std::defret
+  measure-lemma-of-c-sum-merge-lst-lst
+  (<= (count-c-lst updated-c2-lst)
+      (+ (count-c-lst c1-lst)
+         (count-c-lst c2-lst)))
+  :fn c-sum-merge-lst-lst)
+ (std::defret
+  measure-lemma-of-c-sum-merge
+  (<= (+ (count-c-lst c-merged-lst)
+         (count-c-lst to-be-coughed-c-lst))
+      (+ (count-c-lst c1-lst)
+         (count-c-lst c2-lst)))
+  :fn c-sum-merge)
+ (std::defret
+  measure-lemma-of-c-sum-merge-aux
+  (<= (+ (count-c-lst c-merged-lst)
+         (count-c-lst to-be-coughed-c-lst))
+      (+ (count-c-lst c1-lst)
+         (count-c-lst c2-lst)))
+  :fn c-sum-merge-aux)
+ :otf-flg t
+ :hints (("Goal"
+          :do-not-induct t
+          :do-not '(preprocess fertilize generalize)
+          :expand ((C-SUM-MERGE C1-LST C2-LST
+                                :AUTO-SWAP AUTO-SWAP
+                                :CLEAN-C1-LST NIL)
+                   (SINGLE-C-TRY-MERGE SINGLE-C1 SINGLE-C2)
+                   (C-SUM-MERGE-AUX NIL C2-LST :CLEAN-C1-LST CLEAN-C1-LST)
+                   (C-SUM-MERGE C1-LST C2-LST
+                                :AUTO-SWAP AUTO-SWAP
+                                :CLEAN-C1-LST CLEAN-C1-LST)
+                   (C-SUM-MERGE-AUX (MV-NTH 0 (SWAP-C-LSTS C1-LST C2-LST AUTO-SWAP))
+                                    (MV-NTH 1 (SWAP-C-LSTS C1-LST C2-LST AUTO-SWAP))
+                                    :CLEAN-C1-LST CLEAN-C1-LST)
+                   (C-SUM-MERGE-AUX NIL
+                                    (MV-NTH 1 (SWAP-C-LSTS C1-LST C2-LST AUTO-SWAP))
+                                    :CLEAN-C1-LST CLEAN-C1-LST)
+                   (C-SUM-MERGE-AUX (MV-NTH 0 (SWAP-C-LSTS C1-LST C2-LST AUTO-SWAP))
+                                    NIL
+                                    :CLEAN-C1-LST NIL)
+                   (C-SUM-MERGE-AUX (MV-NTH 0 (SWAP-C-LSTS C1-LST C2-LST AUTO-SWAP))
+                                    NIL
+                                    :CLEAN-C1-LST CLEAN-C1-LST)
+                   (C-SUM-MERGE-LST-LST C1-LST C2-LST)
+                   (C-SUM-MERGE-AUX C1-LST C2-LST
+                                    :CLEAN-C1-LST CLEAN-C1-LST)
+                   (C-SUM-MERGE-LST SINGLE-C1 C2-LST)
+                   (C-SUM-MERGE-LST SINGLE-C1 C2-LST)
+                   (C-SUM-MERGE-LST ''0 C2-LST)
+                   (C-SUM-MERGE-LST-AUX SINGLE-C1 C2-LST)
+                   (C-SUM-MERGE-AUX C1-LST NIL :CLEAN-C1-LST NIL)
+                   (C-SUM-MERGE-AUX C1-LST NIL :CLEAN-C1-LST CLEAN-C1-LST))
+          :in-theory (e/d () ()))
+
+         #|("Subgoal *1/20.1"
+          ;:expand (COUNT-C-LST C1-LST) ; ; ;
+         :use ((:instance measure-lemma-of-s-sum-merge-aux ;
+         (s1-lst (CDR C1-LST)) ;
+         (s2-lst (MV-NTH 2 ;
+         (C-SUM-MERGE-LST (CAR C1-LST) ;
+         C2-LST))))) ;
+         :in-theory (disable  measure-lemma-of-s-sum-merge-aux))||#
+
+         #|("Subgoal *1/26"
+         :use ((:instance measure-lemma-of-s-sum-merge-aux
+         (s1-lst (CDR C1-LST))
+         (s2-lst (MV-NTH 2
+         (C-SUM-MERGE-LST (CAR C1-LST)
+         C2-LST)))))
+         :in-theory (disable measure-lemma-of-s-sum-merge-aux))||#
+         ("Subgoal *1/18"
+          :expand ((COUNT-C-LST (LIST SINGLE-C1))
+                   (C-SUM-MERGE-LST SINGLE-C1 C2-LST)
+                   (C-SUM-MERGE-LST-AUX SINGLE-C1 C2-LST))
+          :use ((:instance measure-lemma-of-s-sum-merge-aux
+                           (s1-lst (LIST SINGLE-C1))
+                           (s2-lst C2-LST)))
+          :in-theory (disable measure-lemma-of-s-sum-merge-aux))
+
+         ))
+
+
+
+
+(local
+ (use-arith-5 t))
+
+(verify-guards c-sum-merge-fn
+  :hints (("Goal"
+           :in-theory (e/d (rw-dir2) (rw-dir1)))))
 
 (memoize 'c-sum-merge-aux
          :memo-table-init-size 100000
@@ -49,7 +1277,6 @@
          ;;:recursive nil
          ;;:condition '(and (not (equal c1-lst nil)) (not (equal c2-lst nil)))
          :aokp t)
-
 
 (verify-guards s-of-s-fix-lst-fn)
 
@@ -63,9 +1290,7 @@
 
 (verify-guards c-spec-meta)
 
-
 (verify-guards s-spec-meta-aux)
-
 
 (verify-guards s-spec-meta)
 
